Apply ctr.Put() spec; tweak ghost-state for ctr server to ensure that
own_unused_epoch \ast own_val is contradictory.

src/program_proof/fencing/ctr_proof.v
@@ -23,7 +23,7 @@ Implicit Type γ : ctr_names.
 
 Context `{!mono_natG Σ}.
 Context `{!mapG Σ u64 u64}.
-Context `{!mapG Σ u64 unit}.
+Context `{!mapG Σ u64 bool}.
 
 Definition own_latest_epoch γ (e:u64) (q:Qp) : iProp Σ :=
   mono_nat_auth_own γ.(epoch_gn) q (int.nat e).
@@ -32,10 +32,28 @@ Definition is_latest_epoch_lb γ (e:u64) : iProp Σ :=
   mono_nat_lb_own γ.(epoch_gn) (int.nat e).
 
 Definition own_unused_epoch γ (e:u64) : iProp Σ :=
-  e ⤳[γ.(epoch_token_gn)] ().
+  e ⤳[γ.(epoch_token_gn)] false.
 
 Definition own_val γ (e:u64) (v:u64) (q:Qp): iProp Σ :=
-  e ⤳[γ.(val_gn)]{# q } v.
+  e ⤳[γ.(val_gn)]{# q } v ∗
+  e ⤳[γ.(epoch_token_gn)]□ true.
+
+(* If someone has own_val, that means the ctr sever saw that epoch number, which
+   means the own_unused_epoch was given up. *)
+Lemma unused_own_val_false γ e v q :
+  own_unused_epoch γ e -∗ own_val γ e v q -∗ False.
+Proof.
+Admitted.
+
+Lemma own_val_combine γ e v1 q1 v2 q2 :
+  own_val γ e v1 q1 -∗ own_val γ e v2 q2 -∗ own_val γ e v1 (q1 + q2) ∗ ⌜v1 = v2⌝.
+Proof.
+Admitted.
+
+Lemma own_val_split γ e v q1 q2 :
+  own_val γ e v (q1 + q2) -∗ own_val γ e v q1 ∗ own_val γ e v q2.
+Proof.
+Admitted.
 
 Definition own_Clerk (ck:loc) : iProp Σ.
 Admitted.
@@ -64,45 +82,20 @@ Admitted.
 Lemma wp_Clerk__Put γ ck (e v:u64) :
   ∀ Φ,
   own_Clerk ck -∗
-  (|={⊤,∅}=> ∃ latestEpoch, own_latest_epoch γ latestEpoch (1/2)%Qp ∗
-    if decide (int.Z latestEpoch < int.Z e)%Z then
+  (|={⊤,∅}=> ∃ latestEpoch, if decide (int.Z latestEpoch < int.Z e)%Z then
+      own_latest_epoch γ latestEpoch (1/2)%Qp ∗
       own_unused_epoch γ e ∗
-                            (∀ oldv, own_val γ e v (1/2)%Qp ∗
-                                           own_val γ latestEpoch oldv (1/2)%Qp ∗
+                            (own_val γ e v (1/2)%Qp ∗
+                             (∃ oldv, own_val γ latestEpoch oldv (1/2)%Qp) ∗
                                            own_latest_epoch γ e (1/2)%Qp
-                                           ={∅,⊤}=∗ (own_Clerk ck -∗ Φ #v))
-   else if decide (latestEpoch = e) then
-   ∃ oldv, own_val γ e oldv (1/2)%Qp ∗
-    (own_val γ e v (1/2)%Qp ∗ own_latest_epoch γ e (1/2)%Qp ={∅,⊤}=∗ (own_Clerk ck -∗ Φ #v))
+                                           ={∅,⊤}=∗ (own_Clerk ck -∗ Φ #()))
+   else if decide (int.Z latestEpoch = int.Z e) then
+    ∃ oldv, own_latest_epoch γ latestEpoch (1/2)%Qp ∗
+     own_val γ e oldv (1/2)%Qp ∗
+    (own_val γ e v (1/2)%Qp ∗ own_latest_epoch γ e (1/2)%Qp ={∅,⊤}=∗ (own_Clerk ck -∗ Φ #()))
    else
      True) -∗
-    WP Clerk__Put #ck #e #v {{ Φ }}.
-Proof.
-Admitted.
-
-Lemma wp_Clerk__Get' γ ck (e:u64) :
-  ∀ Φ,
-  own_Clerk ck -∗
-  (|={⊤,∅}=> ∃ latestEpoch, own_latest_epoch γ latestEpoch (1/2)%Qp ∗
-   ∃ v, own_val γ e v (1/2)%Qp ∗
-  ( own_val γ e v (1/2)%Qp ∗
-    own_latest_epoch γ e (1/2)%Qp ∗
-    if decide (int.Z latestEpoch < int.Z e)%Z then
-      own_val γ latestEpoch v (1/2)%Qp
-    else ⌜latestEpoch = e⌝
-    ={∅,⊤}=∗ (own_Clerk ck -∗ Φ #v))) -∗
-    WP Clerk__Get #ck #e {{ Φ }}.
-Proof.
-Admitted.
-
-Lemma wp_Clerk__Get'' γ ck (e:u64) :
-  ∀ Φ,
-  own_Clerk ck -∗
-  (|={⊤,∅}=>
-     (own_unused_epoch γ e ∗ (∃ v, own_val γ e v (1/2)%Qp
-           ={∅,⊤}=∗ (own_Clerk ck -∗ Φ #v))) ∨
-     (∃ v, own_val γ e v (1/2) ∗ (own_val γ e v (1/2) ={∅,⊤}=∗ (own_Clerk ck -∗ Φ #v)))) -∗
-    WP Clerk__Get #ck #e {{ Φ }}.
+    WP Clerk__Put #ck #v #e {{ Φ }}.
 Proof.
 Admitted.
 
